Hashmap/DHashMap/Scratch.lean
@@ -1,0 +1,9 @@
+
+
+theorem evil : Nat = Bool := sorry
+
+def magicBool : Bool := cast evil 4
+def magicNat : Nat := cast evil.symm False
+
+#eval magicNat
+-- #eval magicBool
